James C - yet more reformatting

isabelle/Chapter08_2_Typechecking.thy
@@ -2,22 +2,22 @@ theory Chapter08_2_Typechecking
 imports Chapter08_1_Language
 begin
 
-inductive typecheck :: "type env => expr => type => bool"
-where tc_var [simp]: "lookup gam x = Some t ==> typecheck gam (Var x) t"
-    | tc_str [simp]: "typecheck gam (Str s) StrType"
-    | tc_num [simp]: "typecheck gam (Num n) NumType"
-    | tc_plus [simp]: "typecheck gam e1 NumType ==> typecheck gam e2 NumType ==> 
-                    typecheck gam (Plus e1 e2) NumType"
-    | tc_times [simp]: "typecheck gam e1 NumType ==> typecheck gam e2 NumType ==> 
-                    typecheck gam (Times e1 e2) NumType"
-    | tc_cat [simp]: "typecheck gam e1 StrType ==> typecheck gam e2 StrType ==>
-                    typecheck gam (Cat e1 e2) StrType"
-    | tc_len [simp]: "typecheck gam e StrType ==> typecheck gam (Len e) NumType"
-    | tc_let [simp]: "typecheck gam e1 t1 ==> typecheck (extend gam t1) e2 t2 ==> 
-                    typecheck gam (Let e1 e2) t2"
-    | tc_lam [simp]: "typecheck (extend gam t1) e t2 ==> typecheck gam (Lam t1 e) (Arrow t1 t2)"
-    | tc_appl [simp]: "typecheck gam e1 (Arrow t2 t) ==> typecheck gam e2 t2 ==> 
-                    typecheck gam (Appl e1 e2) t"
+inductive typecheck :: "type env \<Rightarrow> expr \<Rightarrow> type \<Rightarrow> bool" where 
+  tc_var [simp]: "lookup gam x = Some t \<Longrightarrow> typecheck gam (Var x) t"
+| tc_str [simp]: "typecheck gam (Str s) StrType"
+| tc_num [simp]: "typecheck gam (Num n) NumType"
+| tc_plus [simp]: "typecheck gam e1 NumType \<Longrightarrow> typecheck gam e2 NumType \<Longrightarrow>
+    typecheck gam (Plus e1 e2) NumType"
+| tc_times [simp]: "typecheck gam e1 NumType \<Longrightarrow> typecheck gam e2 NumType \<Longrightarrow> 
+    typecheck gam (Times e1 e2) NumType"
+| tc_cat [simp]: "typecheck gam e1 StrType \<Longrightarrow> typecheck gam e2 StrType \<Longrightarrow>
+    typecheck gam (Cat e1 e2) StrType"
+| tc_len [simp]: "typecheck gam e StrType \<Longrightarrow> typecheck gam (Len e) NumType"
+| tc_let [simp]: "typecheck gam e1 t1 \<Longrightarrow> typecheck (extend gam t1) e2 t2 \<Longrightarrow>
+    typecheck gam (Let e1 e2) t2"
+| tc_lam [simp]: "typecheck (extend gam t1) e t2 \<Longrightarrow> typecheck gam (Lam t1 e) (Arrow t1 t2)"
+| tc_appl [simp]: "typecheck gam e1 (Arrow t2 t) \<Longrightarrow> typecheck gam e2 t2 \<Longrightarrow>
+    typecheck gam (Appl e1 e2) t"
 
 inductive_cases [elim!]: "typecheck gam (Var x) t"
 inductive_cases [elim!]: "typecheck gam (Str s) t"
@@ -30,12 +30,11 @@ inductive_cases [elim!]: "typecheck gam (Let e1 e2) t"
 inductive_cases [elim!]: "typecheck gam (Lam t1 e) t"
 inductive_cases [elim!]: "typecheck gam (Appl e1 e2) t"
 
-lemma [simp]: "typecheck gam e t ==> n in gam ==> typecheck (extend_at n gam t') (insert n e) t"
-by (induction gam e t arbitrary: n rule: typecheck.induct, fastforce+)
+lemma [simp]: "typecheck gam e t \<Longrightarrow> n in gam \<Longrightarrow> typecheck (extend_at n gam t') (insert n e) t"
+  by (induction gam e t arbitrary: n rule: typecheck.induct) fastforce+
 
-
-lemma [simp]: "typecheck (extend_at n gam t') e t ==> n in gam ==> typecheck gam e' t' ==> 
-                          typecheck gam (subst e' n e) t"
-by (induction "extend_at n gam t'" e t arbitrary: n gam t' e' rule: typecheck.induct, fastforce+)
+lemma [simp]: "typecheck (extend_at n gam t') e t \<Longrightarrow> n in gam \<Longrightarrow> typecheck gam e' t' \<Longrightarrow>
+    typecheck gam (subst e' n e) t"
+  by (induction "extend_at n gam t'" e t arbitrary: n gam t' e' rule: typecheck.induct) fastforce+
 
 end
