isabelle/Chapter09_1_Language.thy
@@ -14,25 +14,24 @@ datatype expr =
 | Lam type expr
 | Appl expr expr
 
-primrec insert :: "var => expr => expr"
-where "insert n (Var v) = Var (incr n v)"
-    | "insert n Zero = Zero"
-    | "insert n (Suc e) = Suc (insert n e)"
-    | "insert n (Rec et e0 es) = Rec (insert n et) (insert n e0) (insert (next (next n)) es)"
-    | "insert n (Lam t e) = Lam t (insert (next n) e)"
-    | "insert n (Appl e1 e2) = Appl (insert n e1) (insert n e2)"
+primrec insert :: "var \<Rightarrow> expr \<Rightarrow> expr" where 
+  "insert n (Var v) = Var (incr n v)"
+| "insert n Zero = Zero"
+| "insert n (Suc e) = Suc (insert n e)"
+| "insert n (Rec et e0 es) = Rec (insert n et) (insert n e0) (insert (next (next n)) es)"
+| "insert n (Lam t e) = Lam t (insert (next n) e)"
+| "insert n (Appl e1 e2) = Appl (insert n e1) (insert n e2)"
 
-primrec subst :: "expr => var => expr => expr"
-where "subst e' n (Var v) = (if v = n then e' else Var (subr n v))"
-    | "subst e' n Zero = Zero"
-    | "subst e' n (Suc e) = Suc (subst e' n e)"
-    | "subst e' n (Rec et e0 es) = 
-                      Rec (subst e' n et) (subst e' n e0) 
-                          (subst (insert first (insert first e')) (next (next n)) es)"
-    | "subst e' n (Lam t e) = Lam t (subst (insert first e') (next n) e)"
-    | "subst e' n (Appl e1 e2) = Appl (subst e' n e1) (subst e' n e2)"
+primrec subst :: "expr \<Rightarrow> var \<Rightarrow> expr \<Rightarrow> expr" where 
+  "subst e' n (Var v) = (if v = n then e' else Var (subr n v))"
+| "subst e' n Zero = Zero"
+| "subst e' n (Suc e) = Suc (subst e' n e)"
+| "subst e' n (Rec et e0 es) = 
+    Rec (subst e' n et) (subst e' n e0) (subst (insert first (insert first e')) (next (next n)) es)"
+| "subst e' n (Lam t e) = Lam t (subst (insert first e') (next n) e)"
+| "subst e' n (Appl e1 e2) = Appl (subst e' n e1) (subst e' n e2)"
 
-lemma [simp]: "canswap m n ==> insert m (insert n e) = insert (next n) (insert m e)"
-by (induction e arbitrary: n m, simp_all)
+lemma [simp]: "canswap m n \<Longrightarrow> insert m (insert n e) = insert (next n) (insert m e)"
+  by (induction e arbitrary: n m) simp_all
 
 end
