isabelle/Chapter09_2_Typechecking.thy
@@ -2,15 +2,15 @@ theory Chapter09_2_Typechecking
 imports Chapter09_1_Language
 begin
 
-inductive typecheck :: "type env => expr => type => bool"
-where tc_var [simp]: "lookup gam x = Some t ==> typecheck gam (Var x) t"
-    | tc_zero [simp]: "typecheck gam Zero Nat"
-    | tc_suc [simp]: "typecheck gam e Nat ==> typecheck gam (Suc e) Nat"
-    | tc_rec [simp]: "typecheck gam et Nat ==> typecheck gam e0 t ==> 
-                typecheck (extend (extend gam t) Nat) es t ==> typecheck gam (Rec et e0 es) t"
-    | tc_lam [simp]: "typecheck (extend gam t1) e t2 ==> typecheck gam (Lam t1 e) (Arrow t1 t2)"
-    | tc_appl [simp]: "typecheck gam e1 (Arrow t2 t) ==> typecheck gam e2 t2 ==> 
-                typecheck gam (Appl e1 e2) t"
+inductive typecheck :: "type env \<Rightarrow> expr \<Rightarrow> type \<Rightarrow> bool" where 
+  tc_var [simp]: "lookup gam x = Some t \<Longrightarrow> typecheck gam (Var x) t"
+| tc_zero [simp]: "typecheck gam Zero Nat"
+| tc_suc [simp]: "typecheck gam e Nat \<Longrightarrow> typecheck gam (Suc e) Nat"
+| tc_rec [simp]: "typecheck gam et Nat \<Longrightarrow> typecheck gam e0 t \<Longrightarrow> 
+    typecheck (extend (extend gam t) Nat) es t \<Longrightarrow> typecheck gam (Rec et e0 es) t"
+| tc_lam [simp]: "typecheck (extend gam t1) e t2 \<Longrightarrow> typecheck gam (Lam t1 e) (Arrow t1 t2)"
+| tc_appl [simp]: "typecheck gam e1 (Arrow t2 t) \<Longrightarrow> typecheck gam e2 t2 \<Longrightarrow> 
+    typecheck gam (Appl e1 e2) t"
 
 inductive_cases [elim!]: "typecheck gam (Var x) t"
 inductive_cases [elim!]: "typecheck gam Zero t"
@@ -19,11 +19,11 @@ inductive_cases [elim!]: "typecheck gam (Rec et e0 es) t"
 inductive_cases [elim!]: "typecheck gam (Lam t1 e) t"
 inductive_cases [elim!]: "typecheck gam (Appl e1 e2) t"
 
-lemma [simp]: "typecheck gam e t ==> n in gam ==> typecheck (extend_at n gam t') (insert n e) t"
-by (induction gam e t arbitrary: n rule: typecheck.induct, fastforce+)
+lemma [simp]: "typecheck gam e t \<Longrightarrow> n in gam \<Longrightarrow> typecheck (extend_at n gam t') (insert n e) t"
+  by (induction gam e t arbitrary: n rule: typecheck.induct) fastforce+
 
-lemma [simp]: "typecheck (extend_at n gam t') e t ==> n in gam ==> typecheck gam e' t' ==> 
-                          typecheck gam (subst e' n e) t"
-by (induction "extend_at n gam t'" e t arbitrary: n gam t' e' rule: typecheck.induct, fastforce+)
+lemma [simp]: "typecheck (extend_at n gam t') e t \<Longrightarrow> n in gam \<Longrightarrow> typecheck gam e' t' \<Longrightarrow>
+    typecheck gam (subst e' n e) t"
+  by (induction "extend_at n gam t'" e t arbitrary: n gam t' e' rule: typecheck.induct) fastforce+
 
 end
