isabelle/Chapter09_3_Evaluation.thy
@@ -2,68 +2,66 @@ theory Chapter09_3_Evaluation
 imports Chapter09_2_Typechecking
 begin
 
-primrec is_val :: "expr => bool"
-where "is_val (Var v) = False"
-    | "is_val Zero = True"
-    | "is_val (Suc e) = is_val e"
-    | "is_val (Rec et e0 es) = False"
-    | "is_val (Lam t e) = True"
-    | "is_val (Appl e1 e2) = False"
+primrec is_val :: "expr \<Rightarrow> bool" where 
+  "is_val (Var v) = False"
+| "is_val Zero = True"
+| "is_val (Suc e) = is_val e"
+| "is_val (Rec et e0 es) = False"
+| "is_val (Lam t e) = True"
+| "is_val (Appl e1 e2) = False"
 
-inductive eval :: "expr => expr => bool"
-where eval_suc [simp]: "eval e e' ==> eval (Suc e) (Suc e')"
-    | eval_rec_1 [simp]: "eval et et' ==> eval (Rec et e0 es) (Rec et' e0 es)"
-    | eval_rec_2 [simp]: "eval (Rec Zero e0 es) e0"
-    | eval_rec_3 [simp]: "is_val et ==> 
-            eval (Rec (Suc et) e0 es) (subst (Rec et e0 es) first (subst et first es))"
-    | eval_appl_1 [simp]: "eval e1 e1' ==> eval (Appl e1 e2) (Appl e1' e2)"
-    | eval_appl_2 [simp]: "is_val e1 ==> eval e2 e2' ==> eval (Appl e1 e2) (Appl e1 e2')"
-    | eval_appl_3 [simp]: "is_val e2 ==> eval (Appl (Lam t2 e1) e2) (subst e2 first e1)"
+inductive eval :: "expr \<Rightarrow> expr \<Rightarrow> bool" where
+  eval_suc [simp]: "eval e e' \<Longrightarrow> eval (Suc e) (Suc e')"
+| eval_rec_1 [simp]: "eval et et' \<Longrightarrow> eval (Rec et e0 es) (Rec et' e0 es)"
+| eval_rec_2 [simp]: "eval (Rec Zero e0 es) e0"
+| eval_rec_3 [simp]: "is_val et \<Longrightarrow> 
+    eval (Rec (Suc et) e0 es) (subst (Rec et e0 es) first (subst et first es))"
+| eval_appl_1 [simp]: "eval e1 e1' \<Longrightarrow> eval (Appl e1 e2) (Appl e1' e2)"
+| eval_appl_2 [simp]: "is_val e1 \<Longrightarrow> eval e2 e2' \<Longrightarrow> eval (Appl e1 e2) (Appl e1 e2')"
+| eval_appl_3 [simp]: "is_val e2 \<Longrightarrow> eval (Appl (Lam t2 e1) e2) (subst e2 first e1)"
 
-lemma canonical_nat: "is_val e ==> typecheck gam e Nat ==> 
-          e = Zero | (EX e'. e = Suc e' & typecheck gam e' Nat)"
-by (induction e, auto)
+lemma canonical_nat: "is_val e \<Longrightarrow> typecheck gam e Nat \<Longrightarrow> e = Zero \<or> (\<exists>e'. e = Suc e')"
+  by (induction e) auto
 
-lemma canonical_nat_no_vars: "is_val e ==> typecheck gam e Nat ==> typecheck gam' e Nat"
-by (induction e, auto) 
+lemma canonical_nat_no_vars: "is_val e \<Longrightarrow> typecheck gam e Nat \<Longrightarrow> typecheck gam' e Nat"
+  by (induction e) auto
 
-lemma canonical_arrow: "is_val e ==> typecheck gam e (Arrow t1 t2) ==> 
-              EX e'. e = Lam t1 e' & typecheck (extend gam t1) e' t2"
-by (induction e, auto)
+lemma canonical_arrow: "is_val e \<Longrightarrow> typecheck gam e (Arrow t1 t2) \<Longrightarrow> \<exists>e'. e = Lam t1 e'"
+  by (induction e) auto
 
-theorem preservation: "eval e e' ==> typecheck gam e t ==> typecheck gam e' t"
-proof (induction e e' arbitrary: t rule: eval.induct)
-case eval_suc 
-  thus ?case by fastforce
-next case eval_rec_1 
-  thus ?case by fastforce
-next case eval_rec_2 
-  thus ?case by fastforce
-next case (eval_rec_3 et e0 es)
-  from eval_rec_3 canonical_nat_no_vars have "typecheck (extend gam t) (subst et first es) t" by auto
-  with eval_rec_3 show ?case by fastforce
-next case eval_appl_1 
-  thus ?case by fastforce
-next case eval_appl_2 
-  thus ?case by fastforce
-next case eval_appl_3 
-  thus ?case by fastforce
-qed
+theorem preservation: "eval e e' \<Longrightarrow> typecheck gam e t \<Longrightarrow> typecheck gam e' t"
+  proof (induction e e' arbitrary: t rule: eval.induct)
+  case eval_suc 
+    thus ?case by fastforce
+  next case eval_rec_1 
+    thus ?case by fastforce
+  next case eval_rec_2 
+    thus ?case by fastforce
+  next case (eval_rec_3 et e0 es)
+    with canonical_nat_no_vars have "typecheck (extend gam t) (subst et first es) t" by auto
+    with eval_rec_3 show ?case by fastforce
+  next case eval_appl_1 
+    thus ?case by fastforce
+  next case eval_appl_2 
+    thus ?case by fastforce
+  next case eval_appl_3 
+    thus ?case by fastforce
+  qed
 
-theorem progress: "typecheck gam e t ==> gam = empty_env ==> is_val e | (EX e'. eval e e')"
-proof (induction gam e t rule: typecheck.induct)
-case tc_var
-  thus ?case by simp
-next case tc_zero
-  thus ?case by simp
-next case tc_suc
-  thus ?case by (metis eval_suc is_val.simps(3))
-next case tc_rec
-  thus ?case by (metis eval_rec_1 eval_rec_2 eval_rec_3 is_val.simps(3) canonical_nat)
-next case tc_lam
-  thus ?case by simp
-next case tc_appl
-  thus ?case by (metis eval_appl_1 eval_appl_2 eval_appl_3 canonical_arrow)
-qed
+theorem progress: "typecheck gam e t \<Longrightarrow> gam = empty_env \<Longrightarrow> is_val e \<or> (\<exists>e'. eval e e')"
+  proof (induction gam e t rule: typecheck.induct)
+  case tc_var
+    thus ?case by simp
+  next case tc_zero
+    thus ?case by simp
+  next case tc_suc
+    thus ?case by (metis eval_suc is_val.simps(3))
+  next case tc_rec
+    thus ?case by (metis eval_rec_1 eval_rec_2 eval_rec_3 is_val.simps(3) canonical_nat)
+  next case tc_lam
+    thus ?case by simp
+  next case tc_appl
+    thus ?case by (metis eval_appl_1 eval_appl_2 eval_appl_3 canonical_arrow)
+  qed
 
 end
